links: add more definition for keccak air

CoqOfRust/core/array/links/mod.v
@@ -1,7 +1,22 @@
 Require Import CoqOfRust.CoqOfRust.
 Require Import CoqOfRust.links.M.
+Require Import core.array.mod.
+Require Import core.convert.links.mod.
 Require Import core.links.array.
+Require Import core.ops.links.function.
 Require Import core.ops.links.index.
+
+(* pub struct TryFromSliceError(/* private fields */); *)
+Module TryFromSliceError.
+  Parameter t : Set.
+
+  Parameter to_value : t -> Value.t.
+
+  Global Instance IsLink : Link t := {
+    Φ := Ty.path "core::convert::TryFromSliceError";
+    φ := to_value;
+  }.
+End TryFromSliceError.
 
 (*
 impl<T, I, const N: usize> IndexMut<I> for [T; N]
@@ -19,3 +34,60 @@ Module Impl_IndexMut_for_Array.
   Admitted.
 End Impl_IndexMut_for_Array.
 Export Impl_IndexMut_for_Array.
+
+(*
+pub fn from_fn<T, const N: usize, F>(cb: F) -> [T; N]
+where
+    F: FnMut(usize) -> T,
+{
+    try_from_fn(NeverShortCircuit::wrap_mut_1(cb)).0
+}
+*)
+Instance run_from_fn (T : Set) `{Link T} (N : Usize.t) (F : Set) `{Link F}
+    {run_FnMut_for_F : FnMut.Run F Usize.t T}
+    (cb : F) :
+  Run.Trait array.from_fn
+    [φ N] [Φ T; Φ F] [φ cb]
+    (array.t T N).
+Proof.
+  constructor.
+  run_symbolic.
+Admitted.
+
+(*
+impl<'a, T, const N: usize> TryFrom<&'a [T]> for &'a [T; N] {
+    type Error = TryFromSliceError;
+}
+*)
+Module Impl_TryFrom_Ref_for_Ref_Array.
+  Definition Self (T : Set) (N : Usize.t) `{Link T} : Set :=
+    Ref.t Pointer.Kind.Ref (array.t T N).
+
+  Definition Error : Set :=
+    TryFromSliceError.t.
+
+  Instance run (T : Set) `{Link T} (N : Usize.t) :
+    TryFrom.Run (Self T N) (Ref.t Pointer.Kind.Ref (list T)) Error.
+  Admitted.
+End Impl_TryFrom_Ref_for_Ref_Array.
+Export Impl_TryFrom_Ref_for_Ref_Array.
+
+(*
+impl<T, const N: usize> TryFrom<&[T]> for [T; N]
+where
+    T: Copy,
+{
+    type Error = TryFromSliceError;
+*)
+Module Impl_TryFrom_Ref_for_Array.
+  Definition Self (T : Set) (N : Usize.t) `{Link T} : Set :=
+    array.t T N.
+
+  Definition Error : Set :=
+    TryFromSliceError.t.
+
+  Instance run (T : Set) `{Link T} (N : Usize.t) :
+    TryFrom.Run (Self T N) (Ref.t Pointer.Kind.Ref (list T)) Error.
+  Admitted.
+End Impl_TryFrom_Ref_for_Array.
+Export Impl_TryFrom_Ref_for_Array.
