CoqOfRust/plonky3/keccak_air/links/round_flags.v
@@ -1,19 +1,34 @@
 Require Import CoqOfRust.CoqOfRust.
 Require Import CoqOfRust.links.M.
+Require Import core.array.links.mod.
+Require Import core.convert.links.mod.
 Require Import plonky3.air.links.air.
+Require Import plonky3.keccak_air.links.columns.
 Require Import plonky3.keccak_air.round_flags.
 
 (* pub(crate) fn eval_round_flags<AB: AirBuilder>(builder: &mut AB) *)
 Instance run_eval_round_flags
-    {AB : Set} `{Link AB}
-    `{run_AirBuilder_for_AB : AirBuilder.Run AB}
+    {AB : Set} `{Link AB} types
+    `{run_AirBuilder_for_AB : AirBuilder.Run AB types}
     (builder : Ref.t Pointer.Kind.MutRef AB) :
   Run.Trait round_flags.eval_round_flags
     [] [Φ AB] [φ builder]
     unit.
 Proof.
   constructor.
-  run_symbolic_one_step.
-  run_symbolic_one_step.
-  run_symbolic_one_step.
+  destruct run_AirBuilder_for_AB, run_Matrix_for_M.
+  destruct (Impl_Borrow_KeccakCols_for_slice.run types.(AirBuilder.AssociatedTypes.Var)).
+  destruct run_Deref_for_Synthetic2.
+  destruct (Impl_AirBuilder_for_FilteredAirBuilder.run AB types).
+  destruct (
+    let run_TryFrom :=
+      Impl_TryFrom_Ref_for_Array.run
+        types.(AirBuilder.AssociatedTypes.Var) {| Integer.value := 23 |} in
+    Impl_TryInto_for_TryFrom_T.run _ _ _ (run_TryFrom_for_U := run_TryFrom)
+  ).
+  assert (Into.Run types.(AirBuilder.AssociatedTypes.Expr) types.(AirBuilder.AssociatedTypes.Expr)). {
+    apply Impl_Into_for_From_T.run.
+    apply Impl_From_for_T.run.
+  }
+  run_symbolic.
 Admitted.
